More `fold` typeclasses

ADT/Fold.lean
@@ -15,8 +15,16 @@ class FoldlM (γ : Type _) (α : Type _) extends Foldl γ α where
   foldlM {m} [Monad m] {β} : (β → α → m β) → β → γ → m β
 
 class LawfulFoldlM (γ α) [FoldlM γ α] where
-  foldl_eq_foldlM {β} {f : β → α → β} {b : β} {l : γ} :
-  Foldl.foldl f b l = (FoldlM.foldlM (m:=Id) (fun x1 x2 => pure (f x1 x2)) b l).run
+  foldlM_pure {m} [Monad m] [LawfulMonad m] {β} {f : β → α → β} {b : β} {l : γ} :
+    FoldlM.foldlM (m:=m) (fun x1 x2 => pure (f x1 x2)) b l = pure (Foldl.foldl f b l)
+
+class LawfulAppendFoldl (γ α) [Foldl γ α] [Append γ] where
+  foldl_append {β} {f : β → α → β} {b : β} {l l' : γ} :
+    Foldl.foldl f b (l ++ l') = Foldl.foldl f (Foldl.foldl f b l) l'
+
+class LawfulAppendFoldlM (γ : Type u) (α : Type v) [FoldlM γ α] [Append γ] extends LawfulFoldlM γ α where
+  foldlM_append {m : Type w → Type x} [Monad m] [LawfulMonad m] {β} {f : β → α → m β} {b : β} {l l' : γ} :
+    FoldlM.foldlM f b (l ++ l') = FoldlM.foldlM f b l >>= fun b' => FoldlM.foldlM f b' l'
 
 class Foldr (γ : Type _) (α : Type _) where
   foldr {β} : (α → β → β) → β → γ → β
@@ -25,123 +33,154 @@ class FoldrM (γ : Type _) (α : Type _) extends Foldr γ α where
   foldrM {m} [Monad m] {β} : (α → β → m β) → β → γ → m β
 
 class LawfulFoldrM (γ α) [FoldrM γ α] where
-  foldr_eq_foldrM {β} {f : α → β → β} {b : β} {l : γ} :
-  Foldr.foldr f b l = (FoldrM.foldrM (m:=Id) (fun x1 x2 => pure (f x1 x2)) b l).run
+  foldrM_pure {m} [Monad m] [LawfulMonad m] {β} {f : α → β → β} {b : β} {l : γ} :
+    FoldrM.foldrM (m:=m) (fun x1 x2 => pure (f x1 x2)) b l = pure (Foldr.foldr f b l)
+
+class LawfulAppendFoldr (γ α) [Foldr γ α] [Append γ] where
+  foldr_append {β} {f : α → β → β} {b : β} {l l' : γ} :
+    Foldr.foldr f b (l ++ l') = Foldr.foldr f (Foldr.foldr f b l') l
+
+class LawfulAppendFoldrM (γ : Type u) (α : Type v) [FoldrM γ α] [Append γ] extends LawfulFoldrM γ α where
+  foldrM_append {m : Type w → Type x} [Monad m] [LawfulMonad m] {β} {f : α → β → m β} {b : β} {l l' : γ} :
+    FoldrM.foldrM f b (l ++ l') = FoldrM.foldrM f b l' >>= fun b' => FoldrM.foldrM f b' l
+
+theorem LawfulFoldlM.foldl_eq_foldlM {γ α} [FoldlM γ α] [LawfulFoldlM γ α] {β} {f : β → α → β} {b : β} {l : γ} :
+  Foldl.foldl f b l = FoldlM.foldlM (m:=Id) (fun x1 x2 => pure (f x1 x2)) b l := by
+  rw [foldlM_pure]; rfl
+
+theorem LawfulFoldrM.foldr_eq_foldrM {γ α} [FoldrM γ α] [LawfulFoldrM γ α] {β} {f : α → β → β} {b : β} {l : γ} :
+  Foldr.foldr f b l = FoldrM.foldrM (m:=Id) (fun x1 x2 => pure (f x1 x2)) b l := by
+  rw [foldrM_pure]; rfl
+
+instance {γ α} [FoldlM γ α] [Append γ] [LawfulAppendFoldlM.{u, v, w, w} γ α] : LawfulAppendFoldl γ α where
+  foldl_append := by
+    intros
+    simp only [LawfulFoldlM.foldl_eq_foldlM]
+    apply LawfulAppendFoldlM.foldlM_append
+
+instance {γ α} [FoldrM γ α] [Append γ] [LawfulAppendFoldrM.{u, v, w, w} γ α] : LawfulAppendFoldr γ α where
+  foldr_append := by
+    intros
+    simp only [LawfulFoldrM.foldr_eq_foldrM]
+    apply LawfulAppendFoldrM.foldrM_append
 
 instance {α} : FoldlM (List α) α where
   foldl := List.foldl
   foldlM := List.foldlM
 
-instance {α} : LawfulFoldlM (List α) α where
-  foldl_eq_foldlM := List.foldl_eq_foldlM
+instance {α} : LawfulAppendFoldlM (List α) α where
+  foldlM_pure := List.foldlM_pure
+  foldlM_append := List.foldlM_append
 
 instance {α} : FoldrM (List α) α where
   foldr := List.foldr
   foldrM := List.foldrM
 
 instance {α} : LawfulFoldrM (List α) α where
-  foldr_eq_foldrM := List.foldr_eq_foldrM
+  foldrM_pure := List.foldrM_pure
 
 instance {α} : FoldlM (Array α) α where
   foldl := Array.foldl
   foldlM := Array.foldlM
 
-instance {α} : LawfulFoldlM (Array α) α where
-  foldl_eq_foldlM := Array.foldl_eq_foldlM
+instance {α} : LawfulAppendFoldlM (Array α) α where
+  foldlM_pure := Array.foldlM_pure
+  foldlM_append := Array.foldlM_append
 
 instance {α} : FoldrM (Array α) α where
   foldr := Array.foldr
   foldrM := Array.foldrM
 
-instance {α} : LawfulFoldrM (Array α) α where
-  foldr_eq_foldrM := Array.foldr_eq_foldrM
+instance {α} : LawfulAppendFoldrM (Array α) α where
+  foldrM_pure := Array.foldrM_pure
+  foldrM_append := Array.foldrM_append
 
 instance {α} [BEq α] [Hashable α] : FoldlM (HashSet α) α where
   foldl := HashSet.fold
   foldlM := HashSet.foldM
 
 instance {α} [BEq α] [Hashable α] : LawfulFoldlM (HashSet α) α where
-  foldl_eq_foldlM := by
+  foldlM_pure := by
     intros; simp only [Foldl.foldl, FoldlM.foldlM]
     rw [HashSet.fold_eq_foldl_toList, HashSet.foldM_eq_foldlM_toList]
-    apply List.foldl_eq_foldlM
+    apply List.foldlM_pure
 
 instance {α} [Ord α] : FoldlM (TreeSet α) α where
   foldl := TreeSet.foldl
   foldlM := TreeSet.foldlM
 
 instance {α} [Ord α] : LawfulFoldlM (TreeSet α) α where
-  foldl_eq_foldlM := by
+  foldlM_pure := by
     intros; simp only [Foldl.foldl, FoldlM.foldlM]
     rw [TreeSet.foldl_eq_foldl_toList, TreeSet.foldlM_eq_foldlM_toList]
-    apply List.foldl_eq_foldlM
+    apply List.foldlM_pure
 
 instance {α} [Ord α] : FoldrM (TreeSet α) α where
   foldr := TreeSet.foldr
   foldrM := TreeSet.foldrM
 
 instance {α} [Ord α] : LawfulFoldrM (TreeSet α) α where
-  foldr_eq_foldrM := by
+  foldrM_pure := by
     intros; simp only [Foldr.foldr, FoldrM.foldrM]
     rw [TreeSet.foldr_eq_foldr_toList, TreeSet.foldrM_eq_foldrM_toList]
-    apply List.foldr_eq_foldrM
+    apply List.foldrM_pure
 
 instance {α β} [BEq α] [Hashable α] : FoldlM (DHashMap α β) (Sigma β) where
   foldl f := DHashMap.fold (fun s a b => f s ⟨a, b⟩)
   foldlM f := DHashMap.foldM (fun s a b => f s ⟨a, b⟩)
 
 instance {α β} [BEq α] [Hashable α] : LawfulFoldlM (DHashMap α β) (Sigma β) where
-  foldl_eq_foldlM := by
+  foldlM_pure := by
     intros; simp only [Foldl.foldl, FoldlM.foldlM]
     rw [DHashMap.fold_eq_foldl_toList, DHashMap.foldM_eq_foldlM_toList]
-    apply List.foldl_eq_foldlM
+    apply List.foldlM_pure
 
 instance {α β} [Ord α] : FoldlM (DTreeMap α β) (Sigma β) where
   foldl f := DTreeMap.foldl (fun s a b => f s ⟨a, b⟩)
   foldlM f := DTreeMap.foldlM (fun s a b => f s ⟨a, b⟩)
 
 instance {α β} [Ord α] : LawfulFoldlM (DTreeMap α β) (Sigma β) where
-  foldl_eq_foldlM := by
+  foldlM_pure := by
     intros; simp only [Foldl.foldl, FoldlM.foldlM]
     rw [DTreeMap.foldl_eq_foldl_toList, DTreeMap.foldlM_eq_foldlM_toList]
-    apply List.foldl_eq_foldlM
+    apply List.foldlM_pure
 
 instance {α β} [Ord α] : FoldrM (DTreeMap α β) (Sigma β) where
   foldr f := DTreeMap.foldr (fun a b s => f ⟨a, b⟩ s)
   foldrM f := DTreeMap.foldrM (fun a b s => f ⟨a, b⟩ s)
 
 instance {α β} [Ord α] : LawfulFoldrM (DTreeMap α β) (Sigma β) where
-  foldr_eq_foldrM := by
+  foldrM_pure := by
     intros; simp only [Foldr.foldr, FoldrM.foldrM]
     rw [DTreeMap.foldr_eq_foldr_toList, DTreeMap.foldrM_eq_foldrM_toList]
-    apply List.foldr_eq_foldrM
+    apply List.foldrM_pure
 
 instance {α β} [BEq α] [Hashable α] : FoldlM (HashMap α β) (α × β) where
   foldl f := HashMap.fold (fun s a b => f s (a, b))
   foldlM f := HashMap.foldM (fun s a b => f s (a, b))
 
 instance {α β} [BEq α] [Hashable α] : LawfulFoldlM (HashMap α β) (α × β) where
-  foldl_eq_foldlM := by
+  foldlM_pure := by
     intros; simp only [Foldl.foldl, FoldlM.foldlM]
     rw [HashMap.fold_eq_foldl_toList, HashMap.foldM_eq_foldlM_toList]
-    apply List.foldl_eq_foldlM
+    apply List.foldlM_pure
 
 instance {α β} [Ord α] : FoldlM (TreeMap α β) (α × β) where
   foldl f := TreeMap.foldl (fun s a b => f s (a, b))
   foldlM f := TreeMap.foldlM (fun s a b => f s (a, b))
 
 instance {α β} [Ord α] : LawfulFoldlM (TreeMap α β) (α × β) where
-  foldl_eq_foldlM := by
+  foldlM_pure := by
     intros; simp only [Foldl.foldl, FoldlM.foldlM]
     rw [TreeMap.foldl_eq_foldl_toList, TreeMap.foldlM_eq_foldlM_toList]
-    apply List.foldl_eq_foldlM
+    apply List.foldlM_pure
 
 instance {α β} [Ord α] : FoldrM (TreeMap α β) (α × β) where
   foldr f := TreeMap.foldr (fun a b s => f (a, b) s)
   foldrM f := TreeMap.foldrM (fun a b s => f (a, b) s)
 
 instance {α β} [Ord α] : LawfulFoldrM (TreeMap α β) (α × β) where
-  foldr_eq_foldrM := by
+  foldrM_pure := by
     intros; simp only [Foldr.foldr, FoldrM.foldrM]
     rw [TreeMap.foldr_eq_foldr_toList, TreeMap.foldrM_eq_foldrM_toList]
-    apply List.foldr_eq_foldrM
+    apply List.foldrM_pure
